theories/Compositional_Structures/Basic_Modules/Component_Types/Social_Choice_Types/Ballot_Refinement.thy
@@ -236,4 +236,25 @@ proof (-)
 qed
 
 
+
+abbreviation "ballot_impl_assn \<equiv> (arl_assn nat_assn)"
+
+abbreviation "profile_impl_assn \<equiv> (list_assn ballot_impl_assn)"
+
+abbreviation "alts_set_impl_assn \<equiv> (hs.assn nat_assn)"
+
+abbreviation "result_impl_assn \<equiv> alts_set_impl_assn \<times>\<^sub>a alts_set_impl_assn \<times>\<^sub>a alts_set_impl_assn"
+
+definition "alts_assn \<equiv> hr_comp alts_set_impl_assn (\<langle>nat_rel\<rangle>alt_set_rel)"
+
+definition "ballot_assn \<equiv> (hr_comp ballot_impl_assn ballot_rel)"
+
+definition "profile_assn \<equiv> (list_assn ballot_assn)"
+
+abbreviation "result_assn \<equiv> alts_assn \<times>\<^sub>a
+                              alts_assn \<times>\<^sub>a
+                               alts_assn"
+
+
+
 end
